examples/sets/ordSetContainedL.dfy
@@ -1,5 +1,5 @@
 include "../../src/Utils.dfy"
-include "../../src/tree/layer1/OrderedSet.dfy"
+include "../../src/tree/layer1/OrderedSetL.dfy"
 
 
 
@@ -13,7 +13,7 @@ requires forall x | x in s2.Repr() :: allocated(x)
 requires ({s1} + s1.Repr()) !! ({s2}+s2.Repr())
 ensures s1.Valid() && s2.Valid()
 ensures s1.Model()==old(s1.Model()) && s2.Model()==old(s2.Model())
-ensures b == (s1.Model() <= s2.Model())
+ensures b == isSubSet(s1.Model(),s2.Model())
 
 ensures forall x {:trigger x in s1.Repr(), x in old(s1.Repr())} | x in s1.Repr() - old(s1.Repr()) :: fresh(x)
 ensures fresh(s1.Repr()-old(s1.Repr()))
@@ -26,24 +26,21 @@ ensures forall x | x in s2.Repr() :: allocated(x)
 ensures s1.Iterators()>=old(s1.Iterators()) && s2.Iterators()>=old(s2.Iterators())
 {
  var it1:=s1.First(); var x1:int; var x2:int;
- assert it1.Traversed()=={};
  var it2:=s2.First(); b:=true;
- assert it1.Traversed()==it2.Traversed()=={};
  while (it1.HasNext() && it2.HasNext() && b)
-  // decreases s1.Model()+s2.Model()-(it1.Traversed()+it2.Traversed()),b
-   decreases s2.Model()-it2.Traversed(),b
+   decreases |s1.Model()|+|s2.Model()|-(it1.Index()+it2.Index())+(if b then 1 else 0)
    invariant s1.Valid() && s2.Valid() 
    invariant ({s1} + s1.Repr()) !! ({s2}+s2.Repr()) 
    invariant s1.Model()==old(s1.Model()) && s2.Model()==old(s2.Model())
    invariant it1.Valid() && it2.Valid() 
    invariant it1 in s1.Iterators() && it2 in s2.Iterators()
    invariant it1.Parent()==s1 && it2.Parent()==s2
-   invariant it1.Traversed()<=s1.Model() && it2.Traversed()<=s2.Model()
+   invariant 0<=it1.Index()<=|s1.Model()| && 0<=it2.Index()<=|s2.Model()|
    //invariant !it2.HasNext()==> b
-   invariant b ==> it1.Traversed() <= it2.Traversed()
-   invariant !b ==> !(it1.Traversed() <= s2.Model())
-   invariant it1.HasNext() ==> it1.Peek() !in it2.Traversed()
-   invariant forall u | u in it2.Traversed() && it1.Traversed()<s1.Model() :: u<it1.Peek()
+   invariant b ==> isSubSet(s1.Model()[..it1.Index()],s2.Model()[..it2.Index()])
+   invariant !b ==> !isSubSet(s1.Model()[..it1.Index()],s2.Model())
+   invariant it1.HasNext() ==> s1.Model()[it1.Index()] !in s2.Model()[..it2.Index()]
+   invariant forall u::0<=u<it2.Index() && it1.Index()<|s1.Model()| ==> s2.Model()[u]<s1.Model()[it1.Index()]
    
    invariant forall x {:trigger x in s1.Repr(), x in old(s1.Repr())} | x in s1.Repr() - old(s1.Repr()) :: fresh(x)
    invariant forall x {:trigger x in s2.Repr(), x in old(s2.Repr())} | x in s2.Repr() - old(s2.Repr()) :: fresh(x)
@@ -52,23 +49,30 @@ ensures s1.Iterators()>=old(s1.Iterators()) && s2.Iterators()>=old(s2.Iterators(
    invariant s1.Iterators() >= old(s1.Iterators()) && s2.Iterators() >= old(s2.Iterators())
 
  { 
+   assert it1.Index()<|s1.Model()| && it2.Index()<|s2.Model()|;
   if (it1.Peek()==it2.Peek())
   { 
-        x1 := it1.Next(); x2:=it2.Next(); 
+     lmoreSubSet(s1.Model(),s2.Model(),it1.Index(),it2.Index());
+     x1 := it1.Next(); x2:=it2.Next(); 
    
   }
   else if (it1.Peek()<it2.Peek())
    { 
-      assert s2.Model()==it2.Traversed()+(s2.Model()-it2.Traversed());
-     
+     lnotSubSet(s1.Model(),s2.Model(),it1.Index(),it2.Index());
      b:=false;  
      x1:=it1.Next();
     }
   else { 
+    lmoreSubSet2(s1.Model(),s2.Model(),it1.Index(),it2.Index());
     x2 := it2.Next();
     }
   
  }
+ 
+ lSubSet(s1.Model(),s2.Model(),it2.Index());
+ assert b && !it1.HasNext() ==> isSubSet(s1.Model(),s2.Model());
+ assert b && it1.HasNext() ==> !it2.HasNext() && s1.Model()[it1.Index()] !in s2.Model()[..it2.Index()] ==> s1.Model()[it1.Index()] !in s2.Model();
+  
   
   b:=b && !it1.HasNext();
 
