examples/sets/unordSetContained.dfy
@@ -1,10 +1,10 @@
 include "../../src/Utils.dfy"
-include "../../src/tree/layer1/OrderedSet.dfy"
+include "../../src/tree/layer1/UnorderedSet.dfy"
 
 
 
 
-method ordSetContained(s1:OrderedSet,s2:OrderedSet) returns (b:bool)
+method unordSetContained(s1:UnorderedSet,s2:UnorderedSet) returns (b:bool)
 modifies s1, s1.Repr(), s2, s2.Repr()
 requires s1.Valid() && s2.Valid()
 requires forall x | x in s1.Repr() :: allocated(x)
@@ -25,25 +25,19 @@ ensures forall x | x in s2.Repr() :: allocated(x)
 
 ensures s1.Iterators()>=old(s1.Iterators()) && s2.Iterators()>=old(s2.Iterators())
 {
- var it1:=s1.First(); var x1:int; var x2:int;
+ var it1:=s1.First(); var x1:int; var it2:UnorderedSetIterator;
  assert it1.Traversed()=={};
- var it2:=s2.First(); b:=true;
- assert it1.Traversed()==it2.Traversed()=={};
- while (it1.HasNext() && it2.HasNext() && b)
-  // decreases s1.Model()+s2.Model()-(it1.Traversed()+it2.Traversed()),b
-   decreases s2.Model()-it2.Traversed(),b
+  b:=true;
+ while (it1.HasNext() && b)
+   decreases s1.Model()-it1.Traversed(),b
    invariant s1.Valid() && s2.Valid() 
    invariant ({s1} + s1.Repr()) !! ({s2}+s2.Repr()) 
    invariant s1.Model()==old(s1.Model()) && s2.Model()==old(s2.Model())
-   invariant it1.Valid() && it2.Valid() 
-   invariant it1 in s1.Iterators() && it2 in s2.Iterators()
-   invariant it1.Parent()==s1 && it2.Parent()==s2
-   invariant it1.Traversed()<=s1.Model() && it2.Traversed()<=s2.Model()
-   //invariant !it2.HasNext()==> b
-   invariant b ==> it1.Traversed() <= it2.Traversed()
-   invariant !b ==> !(it1.Traversed() <= s2.Model())
-   invariant it1.HasNext() ==> it1.Peek() !in it2.Traversed()
-   invariant forall u | u in it2.Traversed() && it1.Traversed()<s1.Model() :: u<it1.Peek()
+   invariant it1.Valid() 
+   invariant it1 in s1.Iterators() 
+   invariant it1.Parent()==s1 
+   invariant it1.Traversed()<=s1.Model() 
+   invariant b == (it1.Traversed() <= s2.Model())
    
    invariant forall x {:trigger x in s1.Repr(), x in old(s1.Repr())} | x in s1.Repr() - old(s1.Repr()) :: fresh(x)
    invariant forall x {:trigger x in s2.Repr(), x in old(s2.Repr())} | x in s2.Repr() - old(s2.Repr()) :: fresh(x)
@@ -52,25 +46,10 @@ ensures s1.Iterators()>=old(s1.Iterators()) && s2.Iterators()>=old(s2.Iterators(
    invariant s1.Iterators() >= old(s1.Iterators()) && s2.Iterators() >= old(s2.Iterators())
 
  { 
-  if (it1.Peek()==it2.Peek())
-  { 
-        x1 := it1.Next(); x2:=it2.Next(); 
-   
-  }
-  else if (it1.Peek()<it2.Peek())
-   { 
-      assert s2.Model()==it2.Traversed()+(s2.Model()-it2.Traversed());
-     
-     b:=false;  
-     x1:=it1.Next();
-    }
-  else { 
-    x2 := it2.Next();
-    }
-  
- }
-  
-  b:=b && !it1.HasNext();
+   it2 := s2.find(it1.Peek());
+   b := it2.HasNext();
+   x1:=it1.Next();
 
+ }
 }
 
