examples/sets/unordSetIntersection.dfy
@@ -1,0 +1,74 @@
+include "../../src/Utils.dfy"
+include "../../src/tree/layer1/UnorderedSet.dfy"
+
+
+
+
+method unordSetIntersection(s1:UnorderedSet,s2:UnorderedSet,su:UnorderedSet)
+modifies s1, s1.Repr(), s2, s2.Repr(), su, su.Repr()
+requires s1.Valid() && s2.Valid() && su.Valid()
+requires forall x | x in s1.Repr() :: allocated(x)
+requires forall x | x in s2.Repr() :: allocated(x)
+requires forall x | x in su.Repr() :: allocated(x)
+
+requires ({s1} + s1.Repr()) !! ({s2}+s2.Repr())
+requires ({s1} + s1.Repr()) !! ({su}+su.Repr())
+requires ({su} + su.Repr()) !! ({s2}+s2.Repr())
+requires su.Model()=={}
+
+ensures s1.Valid() && s2.Valid() && su.Valid()
+ensures s1.Model()==old(s1.Model()) && s2.Model()==old(s2.Model())
+ensures su.Model() == (s1.Model() * s2.Model())
+
+ensures forall x {:trigger x in s1.Repr(), x in old(s1.Repr())} | x in s1.Repr() - old(s1.Repr()) :: fresh(x)
+ensures fresh(s1.Repr()-old(s1.Repr()))
+ensures forall x | x in s1.Repr() :: allocated(x)
+
+ensures forall x {:trigger x in s2.Repr(), x in old(s2.Repr())} | x in s2.Repr() - old(s2.Repr()) :: fresh(x)
+ensures fresh(s2.Repr()-old(s2.Repr()))
+ensures forall x | x in s2.Repr() :: allocated(x)
+
+ensures forall x {:trigger x in su.Repr(), x in old(su.Repr())} | x in su.Repr() - old(su.Repr()) :: fresh(x)
+ensures fresh(su.Repr()-old(su.Repr()))
+ensures forall x | x in su.Repr() :: allocated(x)
+
+ensures s1.Iterators()>=old(s1.Iterators()) && 
+        s2.Iterators()>=old(s2.Iterators()) &&
+        su.Iterators()>=old(su.Iterators())
+{
+
+ var it1:=s1.First(); var x1:int; var it2: UnorderedSetIterator;
+
+ while (it1.HasNext())
+   decreases (s1.Model()-it1.Traversed())
+   invariant s1.Valid() && s2.Valid() && su.Valid()
+   invariant ({s1} + s1.Repr()) !! ({s2}+s2.Repr()) 
+   invariant ({s1} + s1.Repr()) !! ({su}+su.Repr())
+   invariant ({su} + su.Repr()) !! ({s2}+s2.Repr())
+   invariant s1.Model()==old(s1.Model()) && s2.Model()==old(s2.Model())
+   
+   invariant it1.Valid() 
+   invariant it1 in s1.Iterators() 
+   invariant it1.Parent()==s1 
+   invariant it1.Traversed()<=s1.Model() 
+   invariant su.Model()==it1.Traversed() * s2.Model()
+   
+   invariant forall x {:trigger x in s1.Repr(), x in old(s1.Repr())} | x in s1.Repr() - old(s1.Repr()) :: fresh(x)
+   invariant forall x {:trigger x in s2.Repr(), x in old(s2.Repr())} | x in s2.Repr() - old(s2.Repr()) :: fresh(x)
+   invariant forall x {:trigger x in su.Repr(), x in old(su.Repr())} | x in su.Repr() - old(su.Repr()) :: fresh(x)
+   invariant forall x | x in s1.Repr() :: allocated(x)
+   invariant forall x | x in s2.Repr() :: allocated(x)
+   invariant forall x | x in su.Repr() :: allocated(x)
+   invariant s1.Iterators() >= old(s1.Iterators()) &&
+             s2.Iterators() >= old(s2.Iterators()) &&
+             su.Iterators() >= old(su.Iterators())
+
+{ 
+   it2 := s2.find(it1.Peek());
+   if (it2.HasNext()) 
+     { su.add(it1.Peek()); }
+   x1:=it1.Next();
+ }
+
+}
+
