src/tree/layer1/OrderedSetL.dfy
@@ -1,0 +1,423 @@
+include "../../../src/Utils.dfy"
+
+function isSortedSet(xs:seq<int>):bool
+{forall i,j::0<=i<j<|xs| ==> xs[i]<xs[j]}
+
+
+function isSubSet(xs:seq<int>,ys:seq<int>):bool
+requires isSortedSet(xs) && isSortedSet(ys)
+ensures isSubSet(xs,ys) ==> ((set x | x in xs) <= (set y | y in ys))
+ensures !isSubSet(xs,ys) <== (exists x:: x in xs && x!in ys)
+{ forall x:: x in xs ==> x in ys}
+
+lemma lSubSet(xs:seq<int>,ys:seq<int>,i:int)
+requires 0<=i<=|ys| && isSortedSet(xs) && isSortedSet(ys)
+ensures isSubSet(xs,ys[..i]) ==> isSubSet(xs,ys)
+{}
+
+lemma lmoreSubSet(xs:seq<int>,ys:seq<int>,i:int,j:int)
+requires 0<=i<|xs| && 0<=j<|ys| && isSortedSet(xs) && isSortedSet(ys)
+requires isSubSet(xs[..i],ys[..j]) && xs[i]==ys[j] 
+ensures isSubSet(xs[..i+1],ys[..j+1])
+{assert xs[..i+1]==xs[..i]+[xs[i]];}
+
+lemma lmoreSubSet2(xs:seq<int>,ys:seq<int>,i:int,j:int)
+requires 0<=i<|xs| && 0<=j<|ys| && isSortedSet(xs) && isSortedSet(ys)
+requires isSubSet(xs[..i],ys[..j]) && xs[i]>ys[j] 
+ensures isSubSet(xs[..i],ys[..j+1])
+{}
+
+
+lemma lnotSubSet(xs:seq<int>,ys:seq<int>,i:int,j:int)
+requires 0<=i<|xs| && 0<=j<|ys| && isSortedSet(xs) && isSortedSet(ys)
+requires (forall k::0<=k<j ==> ys[k]<xs[i]) && xs[i]<ys[j] 
+ensures !isSubSet(xs[..i+1],ys)
+{ assert forall k::j<k<|ys| ==> ys[j]<ys[k];
+  assert forall k::j<=k<|ys| ==> xs[i]<ys[k];
+  assert xs[i] in (set x | x in xs[..i+1]) && xs[i] !in (set y | y in ys);
+  }
+
+lemma lnotSubSet2(xs:seq<int>,ys:seq<int>,i:int)//no lo uso
+requires 0<=i<|xs| && isSortedSet(xs) && isSortedSet(ys)
+requires  (forall k::0<=k<|ys| ==> ys[k]<xs[i])
+ensures !isSubSet(xs,ys)
+{assert xs[i] in xs;
+ assert xs[i] !in ys;}
+
+function setSearchAux(xs:seq<int>,x:int,i:int):int
+requires 0<=i<=|xs| &&  isSortedSet(xs) && forall k::i<=k<|xs| ==> x<xs[k]
+ensures 0<=setSearchAux(xs,x,i)<=i 
+ensures forall k::0<=k<setSearchAux(xs,x,i) ==> x>xs[k]
+ensures forall k::setSearchAux(xs,x,i)<=k<|xs| ==> x<=xs[k]
+ensures x in xs ==> 0<=setSearchAux(xs,x,i)<i && xs[setSearchAux(xs,x,i)]==x
+{
+  if (i==0) then 0
+  else if (xs[i-1]==x) then i-1
+  else if (xs[i-1]>x) then setSearchAux(xs,x,i-1)
+  else i//xs[i-1]<x
+   
+}
+
+
+function setSearch(xs:seq<int>,x:int):int
+requires isSortedSet(xs)
+ensures 0<=setSearch(xs,x)<=|xs| 
+ensures forall k::0<=k<setSearch(xs,x) ==> x>xs[k]
+ensures forall k::setSearch(xs,x)<=k<|xs| ==> x<=xs[k]
+ensures x in xs ==> 0<=setSearch(xs,x)<|xs| && xs[setSearch(xs,x)]==x
+{assert xs[..|xs|]==xs;
+  setSearchAux(xs,x,|xs|)
+  
+}
+
+function  SetAdd(xs:seq<int>, x:int):seq<int>
+requires isSortedSet(xs)
+ensures isSortedSet(SetAdd(xs,x))
+ensures (set y | y in xs) + {x} == (set y | y in SetAdd(xs,x)) 
+{
+ if (x in xs) then xs
+ else xs[..setSearch(xs,x)]+[x]+xs[setSearch(xs,x)..]
+}
+
+
+function SetRemove(xs:seq<int>, x:int):seq<int>
+requires isSortedSet(xs)
+ensures isSortedSet(SetRemove(xs,x))
+ensures (set y | y in xs) - {x} == (set y | y in SetRemove(xs,x)) 
+{
+  if (x !in xs) then xs
+  else xs[..setSearch(xs,x)]+xs[setSearch(xs,x)+1..]
+
+}
+
+trait OrderedSetIterator {
+  function Parent(): OrderedSet
+    reads this
+
+  predicate Valid()
+    reads this, Parent(), Parent().Repr()
+
+  function Index(): nat
+    reads this, Parent(), Parent().Repr()
+    requires Valid()
+    requires Parent().Valid()
+    ensures Index() <= |Parent().Model()|
+
+  function method HasNext(): bool
+    reads this, Parent(), Parent().Repr()
+    requires Valid()
+    requires Parent().Valid()
+    ensures HasNext() <==> Index() < |Parent().Model()|
+
+  function method HasPrev(): bool
+    reads this, Parent(), Parent().Repr()
+    requires Valid()
+    requires Parent().Valid()
+    ensures HasPrev() <==> Index() > 0
+
+  method Next() returns (x: int)
+    modifies this
+    requires Valid()
+    requires Parent().Valid()
+    requires HasNext()
+    requires allocated(Parent())
+    requires forall it | it in Parent().Repr() :: allocated(it)
+    ensures Parent().Valid()
+    ensures Valid()
+    ensures old(Parent()) == Parent()
+    ensures old(Parent().Model()) == Parent().Model()
+
+    ensures forall x {:trigger x in Parent().Repr(), x in old(Parent().Repr())} | x in Parent().Repr() - old(Parent().Repr()) :: fresh(x)
+    ensures fresh(Parent().Repr()-old(Parent().Repr()))
+    ensures forall x | x in Parent().Repr() :: allocated(x)
+
+    ensures Parent().Iterators() == old(Parent().Iterators())
+    ensures x == Parent().Model()[old(Index())]
+    ensures Index() == 1 + old(Index())
+    ensures forall it | it in Parent().Iterators() && old(it.Valid()) ::
+      it.Valid() && (it != this ==> it.Index() == old(it.Index()))
+
+  method Prev() returns (x: int)
+    modifies this
+    requires Valid()
+    requires Parent().Valid()
+    requires HasPrev() && HasNext()
+    requires allocated(Parent())
+    requires forall it | it in Parent().Repr() :: allocated(it)
+    ensures Parent().Valid()
+    ensures Valid()
+    ensures old(Parent()) == Parent()
+    ensures old(Parent().Model()) == Parent().Model()
+
+    ensures forall x {:trigger x in Parent().Repr(), x in old(Parent().Repr())} | x in Parent().Repr() - old(Parent().Repr()) :: fresh(x)
+    ensures fresh(Parent().Repr()-old(Parent().Repr()))
+    ensures forall x | x in Parent().Repr() :: allocated(x)
+
+    ensures Parent().Iterators() == old(Parent().Iterators())
+    ensures x == Parent().Model()[old(Index())]
+    ensures Index() == old(Index()) - 1
+    ensures forall it | it in Parent().Iterators() && old(it.Valid()) ::
+      it.Valid() && (it != this ==> it.Index() == old(it.Index()))
+
+  function method Peek(): int
+    reads this, Parent(), Parent().Repr()
+    requires Valid()
+    requires Parent().Valid()
+    requires HasNext()
+    ensures Peek() == Parent().Model()[Index()]
+
+  method Copy() returns (it: OrderedSetIterator)
+    modifies Parent(), Parent().Repr()
+    requires Valid()
+    requires Parent().Valid()
+    requires allocated(Parent())
+    requires forall it | it in Parent().Iterators() :: allocated(it)
+    ensures fresh(it)
+    ensures Valid()
+    ensures Parent() == old(Parent())
+    ensures Parent().Valid()
+    ensures Parent().Model() == old(Parent().Model())
+
+    ensures forall x {:trigger x in Parent().Repr(), x in old(Parent().Repr())} | x in Parent().Repr() - old(Parent().Repr()) :: fresh(x)
+    ensures fresh(Parent().Repr()-old(Parent().Repr()))
+    ensures forall x | x in Parent().Repr() :: allocated(x)
+    
+    ensures it.Valid()
+    ensures Parent().Iterators() == {it} + old(Parent().Iterators())
+    ensures Parent() == it.Parent()
+    ensures Index() == it.Index()
+    ensures forall it | it in old(Parent().Iterators()) && old(it.Valid()) ::
+      it.Valid() && it.Index() == old(it.Index())
+
+  
+}
+
+trait OrderedSet {
+  function ReprDepth(): nat
+    ensures ReprDepth() > 0
+
+  function ReprFamily(n: nat): set<object>
+    decreases n
+    requires n <= ReprDepth()
+    ensures n > 0 ==> ReprFamily(n) >= ReprFamily(n-1)
+    reads this, if n == 0 then {} else ReprFamily(n-1)
+
+  function Repr(): set<object>
+    reads this, ReprFamily(ReprDepth()-1)
+  {
+    ReprFamily(ReprDepth())
+  }
+
+  lemma UselessLemma()
+    ensures Repr() == ReprFamily(ReprDepth());
+
+  predicate Valid()
+    reads this, Repr()
+
+  function Model(): seq<int>
+    reads this, Repr()
+    requires Valid()
+    ensures isSortedSet(Model())
+
+  function method Empty(): bool
+    reads this, Repr()
+    requires Valid()
+    ensures Empty() <==> Model() == []
+
+  function method Size(): nat
+    reads this, Repr()
+    requires Valid()
+    ensures Size() == |Model()|
+
+  function Iterators(): set<OrderedSetIterator>
+    reads this, Repr()
+    requires Valid()
+    ensures forall it | it in Iterators() :: it in Repr() && it.Parent() == this
+
+method First() returns (it: OrderedSetIterator)
+    modifies this, Repr()
+    requires Valid()
+    requires forall x | x in Repr() :: allocated(x)
+    ensures Valid()
+    ensures Model() == old(Model())
+
+    ensures forall x {:trigger x in Repr(), x in old(Repr())} | x in Repr() - old(Repr()) :: fresh(x)
+    ensures fresh(Repr()-old(Repr()))
+    ensures forall x | x in Repr() :: allocated(x)
+
+    ensures fresh(it)
+    ensures Iterators() == {it} + old(Iterators())
+    ensures it.Valid()
+    ensures it.Index() == 0
+    ensures it.Parent() == this
+    ensures forall it | it in old(Iterators()) && old(it.Valid()) ::
+      it.Valid() && it.Index() == old(it.Index())
+
+  method Last() returns (it: OrderedSetIterator)//iterator to the last element
+    modifies this, Repr()
+    requires Valid()
+    requires forall x | x in Repr() :: allocated(x)
+    ensures Valid()
+    ensures Model() == old(Model())
+
+    ensures forall x {:trigger x in Repr(), x in old(Repr())} | x in Repr() - old(Repr()) :: fresh(x)
+    ensures fresh(Repr()-old(Repr()))
+    ensures forall x | x in Repr() :: allocated(x)
+
+    ensures fresh(it)
+    ensures Iterators() == {it} + old(Iterators())
+    ensures it.Valid()
+    ensures if |Model()|==0 then it.Index() == 0 
+            else it.Index() == |Model()|-1
+    ensures it.Parent() == this
+    ensures forall it | it in old(Iterators()) && old(it.Valid()) ::
+      it.Valid() && it.Index() == old(it.Index())
+
+  method contains(x:int) returns (b:bool)
+    requires Valid()
+    ensures Valid() && b == (x in Model())
+
+  method add(x:int)
+    modifies this,Repr()
+    requires Valid()
+    requires forall x | x in Repr() :: allocated(x)
+    ensures Valid()
+    ensures Model()==SetAdd(old(Model()),x)  
+
+    ensures forall x {:trigger x in Repr(), x in old(Repr())} | x in Repr() - old(Repr()) :: fresh(x)
+    ensures fresh(Repr()-old(Repr()))
+    ensures forall x | x in Repr() :: allocated(x)
+   
+    ensures Iterators() == old(Iterators())
+
+
+
+  method remove(x:int) 
+    modifies this,Repr()
+    requires Valid()
+    requires forall x | x in Repr() :: allocated(x)
+    ensures Valid()
+    ensures Model()==SetRemove(old(Model()),x)  
+
+    ensures forall x {:trigger x in Repr(), x in old(Repr())} | x in Repr() - old(Repr()) :: fresh(x)
+    ensures fresh(Repr()-old(Repr()))
+    ensures forall x | x in Repr() :: allocated(x)
+
+    ensures Iterators() == old(Iterators())
+
+
+  method find(x:int) returns (newt:OrderedSetIterator)
+    requires Valid()
+    requires forall x | x in Repr() :: allocated(x)
+    ensures Valid() 
+    ensures fresh(newt) 
+    ensures newt.Valid() && newt.Parent()==this
+    ensures x in Model() ==> 0<=newt.Index()<|Model()| && Model()[newt.Index()]==x
+    ensures x !in Model() ==> newt.Index()==|Model()|
+
+    ensures forall x {:trigger x in Repr(), x in old(Repr())} | x in Repr() - old(Repr()) :: fresh(x)
+    ensures fresh(Repr()-old(Repr()))
+    ensures forall x | x in Repr() :: allocated(x)
+    ensures Iterators() == {newt}+old(Iterators())
+
+  method insert(mid: OrderedSetIterator, x: int) returns (newt:OrderedSetIterator)
+    modifies this, Repr()
+    requires Valid()
+    requires mid.Valid() 
+    //mid just a hint, it is inserted where corresponds
+    //efficiently or not if it respects order
+    requires mid.Parent() == this
+    requires mid in Iterators()
+    requires forall x | x in Repr() :: allocated(x)
+    ensures Valid()
+    ensures Model() == SetAdd(old(Model()), x)
+
+    ensures forall x {:trigger x in Repr(), x in old(Repr())} | x in Repr() - old(Repr()) :: fresh(x)
+    ensures fresh(Repr()-old(Repr()))
+    ensures forall x | x in Repr() :: allocated(x)
+
+    ensures fresh(newt)
+    ensures Iterators() == {newt}+old(Iterators())
+    ensures newt.Valid() && newt.Parent()==this
+    ensures newt.HasNext() && Model()[newt.Index()]==x
+    //points either to the inserted elemento or to the already existing one
+ 
+
+
+  method erase(mid:OrderedSetIterator) returns (next: OrderedSetIterator)
+    modifies this, Repr()
+    requires Valid()
+    requires mid.Valid()
+    requires mid.Parent() == this
+    requires mid.HasNext()
+    requires mid in Iterators()
+    requires forall x | x in Repr() :: allocated(x)
+    ensures Valid()
+    ensures Model()==SetRemove(old(Model()),old(Model())[old(mid.Index())])
+    
+    ensures fresh(next)
+    ensures Iterators() == {next}+old(Iterators())
+    ensures next.Valid() && next.Parent()==this && next.Index()==old(mid.Index())
+}
+
+
+
+method {:verify false} try(s:OrderedSet)
+modifies s, s.Repr()
+requires s.Valid() && s.Empty()
+requires forall x | x in s.Repr() :: allocated(x)
+ensures s.Valid()
+ensures forall x {:trigger x in s.Repr(), x in old(s.Repr())} | x in s.Repr() - old(s.Repr()) :: fresh(x)
+ensures fresh(s.Repr()-old(s.Repr()))
+ensures forall x | x in s.Repr() :: allocated(x)
+{
+ /*s.add(3);
+ s.add(4);
+ assert 3 in s.Model();
+ assert 4 in s.Model();
+ assert (set x | x in s.Model()) == {3,4};
+ s.add(4);
+ assert (set x | x in s.Model()) == {3,4};
+ s.remove(2);
+  assert (set x | x in s.Model()) == {3,4};
+ s.remove(3);
+  assert (set x | x in s.Model()) == {4};
+ s.remove(4);
+   assert (set x | x in s.Model()) == {};*/
+ s.add(2); s.add(7); s.add(0); s.add(1);s.add(10);
+
+ var b:=s.contains(10);
+ assert b;
+
+ var it:=s.First(); var cont:=0;
+  while (it.HasNext())
+  decreases |s.Model()|-it.Index()
+  invariant it.Valid() && it.Parent()==s
+  invariant s.Valid()
+  invariant  forall x {:trigger x in s.Repr(), x in old(s.Repr())} | x in s.Repr() - old(s.Repr()) :: fresh(x)
+  invariant fresh(s.Repr()-old(s.Repr()))
+  invariant forall x | x in s.Repr() :: allocated(x)
+    {var aux:=it.Next();
+     if (aux%2==0) {cont:=cont+1;} 
+    } 
+  var it2:=s.find(2);
+  assert it2.Index()==4;
+  it2:=s.find(7); 
+  assert it.Index()==3;  
+  var aux:=it.Next();
+  assert aux==7;assert it.Index()==4;
+  
+  var it3:=s.find(7);
+  it3:=s.insert(it3,5);//efficient
+  assert it3.Index()==3;
+  it3:=s.insert(it3,12);
+  assert it3.Index()==5;
+  var z:=it3.Prev();
+  assert it3.Index()==4;
+
+  var it4:=s.Last();
+  z:=it4.Prev();
+  z:=it4.Prev();
+
+  assert z==10;
+}
